\section{Examples}


\paragraph{Booleans}
$$
\begin{array}{lllll}
  \text{Bool}
  &:=& \Pi \alpha^* . \alpha\to\alpha\to\alpha
  &:& *
  \\
  \text{true}
  &:=& \lambda \alpha^* x^\alpha y^\alpha . x
  &:& \text{Bool}
  \\
  \text{false}
  &:=& \lambda \alpha^* x^\alpha y^\alpha . y
  &:& \text{Bool}
\end{array}
$$


\paragraph{Pairs}

$$
\begin{array}{lllll}
  P
  &:=& \lambda \alpha^* \beta^*
       . \Pi \gamma^*
       . (\alpha\to\beta\to\gamma) \to \gamma
  &:& *
  \\
  \text{pair}
  &:=& \lambda
       \alpha^*
       \beta^*
       a^\alpha
       b^\beta
       \gamma^*
       f^{\alpha\to\beta\to\gamma}
       . f a b
  &:& \Pi \alpha^* \beta^* a^\alpha b^\beta . P \alpha \beta
  \\
  \pi_1
  &:=& \lambda
       \alpha^*
       \beta^*
       p^{P\alpha\beta}
       . p \alpha (\lambda a^\alpha b^\beta. a)
  &:& \Pi \alpha^* \beta^* (P\alpha\beta)^* . \alpha
  \\
  \pi_2
  &:=& \lambda
       \alpha^*
       \beta^*
       p^{P\alpha\beta}
       . p \beta (\lambda a^\alpha b^\beta. b)
  &:& \Pi \alpha^* \beta^* (P\alpha\beta)^* . \beta
\end{array}
$$



\paragraph{Natural numbers}
$$
\begin{array}{lllll}
  \Nat
  &:= & \Pi \alpha^* . (\alpha \to \alpha) \to \alpha \to \alpha
  &:& *
  \\
  0
  &:=& \lambda \alpha^* f^{\alpha\to\alpha} z^\alpha. z
  &:& \Nat
  \\
  (')
  &:=& \lambda p^\Nat \alpha^* f^{\alpha\to\alpha} z^\alpha . f (p \alpha f z)
  &:& \Nat\to\Nat
\end{array}
$$

Primitiv recursion is done with two functions $g:\tau$ and
$h:\Nat \to \tau \to \tau$. We need a step function which takes the type
$\tau$ and the function $h$ and returns a function with the type
$\text{Pair}\,\Nat\,\tau \to \text{Pair}\,\Nat\,\tau$.
$$
\begin{array}{lll}
  \text{start}
  &:=& \lambda
       \alpha^*
       g^\alpha
       . \text{pair}\,\Nat\,\alpha\,0\,g
  \\
  & &: \Pi \alpha^*. \alpha \to P\Nat\alpha
  \\
  \text{step}
  &:=& \lambda
       \alpha^*
       h^{\Nat\to\alpha\to\alpha}
       p^{P\Nat\alpha}
       . \text{pair}\,\Nat\,\alpha\,
       (\pi_1\,p)'\,
       (h (\pi_1 p) (\pi_2 p)
  \\
  & &: \Pi \alpha^* (\Nat\to\alpha\to\alpha)
      . (P\Nat\alpha)\to (P\Nat\alpha)
\end{array}
$$


Predecessor function
$$
\text{pred} :=
\lambda n^\Nat.
\pi_2 (
  n
  \Nat (\text{step}\,\Nat (\lambda n^\Nat \_^\Nat. n))
  (\text{pair}\,\Nat\,\Nat\,0\,0)
)
$$



\paragraph{Lists}

$$
\begin{array}{lllll}
  L
  &:=& \lambda \alpha^* .
       \Pi \beta^* . (\alpha\to\beta\to\beta) \to \beta \to \beta
  &:& * \to *
  \\
  \text{nil}
  &:=& \lambda \alpha^* \beta^* f^{(\alpha\to\beta\to\beta)} s^\beta . s
  &:& \Pi \alpha^* . L \alpha
  \\
  \text{cons}
  &:=& \lambda
       \alpha^*
       h^\alpha
       t^{L\alpha}
       \beta^*
       f^{(\alpha\to\beta\to\beta)}
       s^\beta
       . f h (t \beta f s)
  &:& \Pi \alpha^* . \alpha \to L \alpha \to L \alpha
\end{array}
$$




\paragraph{Trees}

$$
\begin{array}{lllll}
  T
  &:=& \lambda \alpha^* .
       \Pi \beta^* . (\alpha\to\beta\to\beta\to\beta) \to \beta \to \beta
  &:& * \to *
  \\
  \text{empty}
  &:=& \lambda \alpha^* \beta^* f^{\alpha\to\beta\to\beta\to\beta} e^\beta . e
  &:& \Pi \alpha^* . T \alpha
  \\
  \text{node}
  &:=& \lambda
       \alpha^*
       a^\alpha
       l^{T\alpha}
       r^{T\alpha}
       \beta^*
       f^{\alpha\to\beta\to\beta\to\beta}
       e^\beta
       . f a (l \beta f e) (r \beta f e)
  &:& \Pi \alpha^* . \alpha \to T \alpha \to T \alpha \to T \alpha
\end{array}
$$

%%% Local Variables:
%%% mode: latex
%%% TeX-master: "0typed"
%%% End:
